pcuic/theories/PCUICCumulativity.v
@@ -134,6 +134,22 @@ Proof.
   inversion 1; reflexivity.
 Qed.
 
+Lemma eq_term_eq_term_napp {cf:checker_flags} Σ ϕ napp t t' :
+  eq_term Σ ϕ t t' -> 
+  eq_term_upto_univ_napp Σ (eq_universe ϕ) (eq_universe ϕ) napp t t'.
+Proof.
+  intros. eapply eq_term_upto_univ_impl. 5:eauto.
+  4:auto with arith. all:typeclasses eauto.
+Qed.
+
+Lemma leq_term_leq_term_napp {cf:checker_flags} Σ ϕ napp t t' :
+  leq_term Σ ϕ t t' -> 
+  eq_term_upto_univ_napp Σ (eq_universe ϕ) (leq_universe ϕ) napp t t'.
+Proof.
+  intros. eapply eq_term_upto_univ_impl. 5:eauto.
+  4:auto with arith. all:typeclasses eauto.
+Qed.
+
 Lemma eq_term_mkApps `{checker_flags} Σ φ f l f' l' :
   eq_term Σ φ f f' ->
   All2 (eq_term Σ φ) l l' ->
@@ -142,7 +158,7 @@ Proof.
   induction l in l', f, f' |- *; intro e; inversion_clear 1.
   - assumption.
   - cbn. eapply IHl.
-    + constructor; assumption.
+    + constructor; auto. now apply eq_term_eq_term_napp.
     + assumption.
 Qed.
 
@@ -162,6 +178,7 @@ Proof.
   - assumption.
   - cbn. apply IHl.
     + constructor; try assumption.
+      now eapply leq_term_leq_term_napp.
     + assumption.
 Qed.
 
@@ -255,7 +272,7 @@ Proof.
   intros Σ Γ f g x h.
   induction h.
   - eapply cumul_refl. constructor.
-    + assumption.
+    + apply leq_term_leq_term_napp. assumption.
     + apply eq_term_refl.
   - eapply cumul_red_l ; try eassumption.
     econstructor. assumption.
